#notes

By [[Euler's Formula]], $e^{i\theta}=\cos \theta+i\sin \theta$
So, say $\theta \to-\theta$: $e^{-i\theta}=\cos \theta-i\sin \theta$
$$\implies \cos \theta=\frac{e^{i\theta}+e^{-i\theta}}{2},\space \sin \theta=\frac{e^{i\theta}-e^-i\theta}{2i}$$
Note that they are similar to the hyperbolic formulae, but ==not the same==!
## Derivations
$$\cos^2\theta=(\frac{e^{i\theta}+e^{-i\theta}}{2})^2=\frac{(e^i\theta)^2+2e^{i\theta}e^{-i\theta}+(e^{-i\theta})^2}{4}$$$$=\frac{e^{2i\theta}+2+e^{-2i\theta}}{4}=\frac{1}{2}\left( \frac{e^{2i\theta}+e^{-2i\theta}}{2} \right)+\frac{1}{2}=\frac{1}{2}\cos 2\theta+\frac{1}{2}$$
But also: $$\cos^4\theta=(\frac{e^{i\theta}+e^{-i\theta}}{2})^4=\dots\text{ Use Binomia expansion: 14641}$$$$=\frac{1}{16}(e^{4i\theta}+4e^{2i\theta}+6+4e^{-2i\theta}+e^{-4i\theta})$$$$=\frac{1}{16}(2\cos 4\theta+8\cos 2\theta+6)$$So, $$\cos^4\theta=\frac{1}{8}\cos 4\theta+\frac{1}{2}\cos 2\theta + \frac{3}{8}$$

