#definition 

$$
\eqalign{
F_{l \wedge m} &= \{ \{ \bar{l},\bar{m},x_{l\wedge m} \},\{ l,\overline{x_{l\wedge m}} \},\{ m,\overline{x_{l\wedge m}} \} \} \\
F_{l \vee m} &= \{ \{ \bar{l},x_{l\vee m} \},\{ \bar{m},x_{l\vee m} \},\{ l,m,\overline{x_{l\vee m}} \} \} \\
F_{l \implies m} &= \{ \{ l,x_{l \implies m} \},\{ \bar{m},x_{l \implies m} \},\{ \bar{l},m,\overline{x_{l \implies m}} \} \} \\
F_{l \iff m} &= \{ \{ l, m, x_{l \iff m} \},\{ \bar{l},\bar{m},x_{l \iff m} \},\{ \bar{l},m,\overline{x_{l \iff m}} \},\{ l,\bar{m},\overline{x_{l \iff m}} \} \} \\
F_{l \oplus m} &= \{ \{ \bar{l},m,x_{l \oplus m} \},\{ l,\bar{m},x_{l \oplus m} \},\{ l,m,\overline{x_{l \oplus m}} \},\{ \bar{l},\bar{m},\overline{x_{l \oplus m}} \} \} \\
}
$$
